## Ejercicio 18
- Sea:
```
1.{¬Progenitor(X,Y), Descendiente(Y,X)} 
2.{¬Descendiente(X,Y), ¬Descendiente(Y,Z), Descendiente(X,Z)}
3.{¬Abuelo(X,Y), Progenitor(X, medio(X,Y))} 
4.{¬Abuelo(X,Y), Progenitor(medio(X,Y), Y)}
```
- Demostrar:
```
5. ∀X.∀Y.(Abuelo(X,Y) => Descendiente(Y,X))
```

- Quiero ver que:
```
(1 ∧ 2 ∧ 3 ∧ 4 => 5)

Niego la formula y uso resolucion:
¬(1 ∧ 2 ∧ 3 ∧ 4 => 5) =
(1 ∧ 2 ∧ 3 ∧ 4) ∧ ¬5

¬5 = ¬(∀X.∀Y.(Abuelo(X,Y) => Descendiente(Y,X)))

Saco implicación:
¬(∀X.∀Y.(¬Abuelo(X,Y) v Descendiente(Y,X)))

Forma normal negada:
∃X.∃Y.¬(¬Abuelo(X,Y) v Descendiente(Y,X)) =
∃X.∃Y.(Abuelo(X,Y) ∧ ¬Descendiente(Y,X))

Skolemizo:
(Abuelo(c,d) ∧ ¬Descendiente(d,c))

Forma clausal:
5 = {{Abuelo(c,d)}, {¬Descendiente(d,c)}}
```
- Ahora uso resolución general:
```
1.{¬Progenitor(X1,Y1), Descendiente(Y1,X1)} 
2.{¬Descendiente(X2,Y2), ¬Descendiente(Y2,Z2), Descendiente(X2,Z2)}
3.{¬Abuelo(X3,Y3), Progenitor(X3, medio(X3,Y3))} 
4.{¬Abuelo(X4,Y4), Progenitor(medio(X4,Y4), Y4)}
5.{Abuelo(c,d)}
6.{¬Descendiente(d,c)}

De 5 y 3 con {X3 := a, Y3 := b}:
  7: {progenitor(a,medio(a,b))}

De 7 y 1 con {X1 := a, Y1 := medio(a,b)}:
  8: {descendiente(medio(a,b),a)}

De 8 y 2 con {Y2 := medio(a,b), Z2 := a}:
  9: {¬descendiente(X2,medio(a,b)), descendiente(X2,a)}

De 9 y 1 con {Y1 := X2, X1 := medio(a,b)}:
  10: {¬progenitor(medio(a,b),X2), descendiente(X2,a)}

De 4 y 10 con {Y4 := b, X4 := a, X2 := b}:
  11: {¬abuelo(a,b), descendiente(b,a)}

De 11 y 5 con {}:
  12: {descendiente(b,a)}

De 12 y 6 con {}:
  13: {}

```