## Ejercicio 3:
### I:
```prolog
σ = (P ⇒ (P ⇒ Q)) ⇒ (P ⇒ Q)

¬σ = ¬((P ⇒ (P ⇒ Q)) ⇒ (P ⇒ Q))

CNF: ¬(¬(P => (P => Q) v (P => Q))) =
     ¬(¬(¬P v (¬P v Q)) v (¬P v Q)) =
       (¬P v (¬P v Q)) ∧ ¬(¬P v Q)  =
       (¬P v Q) ∧ P ∧ ¬Q

C = {{¬P,Q},{P},{¬Q}}

De 1 y 2 obtengo 4 = {Q}
De 3 y 4 obtengo 5 = {}

Luego C ⊢ ⊥
Luego ¬σ ⊢ ⊥.
Luego ⊢ σ


```
### II:
```prolog
(R ⇒ ¬Q) ⇒ ((R ∧ Q) ⇒ P )

¬σ = ¬((R => ¬Q) => ((R ∧ Q) => P))

CNF: ¬(¬(¬R v ¬Q) v (¬(R ∧ Q) v P)) =
     (¬R v ¬Q) ∧ ¬((¬R v ¬Q) v P)   =
     (¬R v ¬Q) ∧ R ∧ Q ∧ ¬P

C = {{¬R,¬Q},R,Q,¬P}

De 1 y 2 obtengo 5 = {¬Q}
De 5 y 3 obtengo 6 = {}

Luego C ⊢ ⊥
Luego ¬σ ⊢ ⊥.
Luego ⊢ σ
```

### III:
```prolog
((P ⇒ Q) ⇒ (R ⇒ ¬Q)) ⇒ ¬(R ∧ Q)

¬σ = ¬((P => Q) => (R => ¬Q) => ¬(R ∧ Q))

CNF: ¬(¬((P => Q) => (R => ¬Q) v ¬(R ∧ Q)))  =
      ((P => Q) => (R => ¬Q)) ∧ (R ∧ Q)      =
      (¬(¬P v Q) v (¬R v ¬Q)) ∧ (R ∧ Q)      =
      (P ∧ ¬Q v (¬R v ¬Q) ∧ R ∧ Q)

C = {{P}, {¬Q}, {¬R,¬Q}, {R}, {Q}}

De 2 y 5 obtengo {}

Luego C ⊢ ⊥
Luego ¬σ ⊢ ⊥.
Luego ⊢ σ

```

