## Ejercicio 6
### I:
```prolog
Skolem:
∃X.∃Y.X < Y
∃Y. c1 < Y
c1 < c2

Causal:
{c1 < c2}
```

### II:
```prolog
Skolem
∀X.∃Y.X < Y
∀X. X < f(X)

Causal:
{X < f(X)}
```

### III:
```prolog
∀X.¬(P(X) ∧ ∀Y.(¬P(Y) ∨ Q(Y)))

Skolem:
∀X.¬P(X) v ¬∀Y.(¬P(Y) ∨ Q(Y))
∀X.¬P(X) v ∃Y.¬(¬P(Y) ∨ Q(Y))
∀X.¬P(X) v (P(f(X) ∧ ¬Q(f(X))))
∀X.(¬P(X) v P(f(X))) ∧ (¬P(X) v ¬Q(f(X)))

Causal:
{{¬P(X),P(f(X))}, {¬P(X), ¬Q(f(X))}}

```

### IV:
```prolog
∃X.∀Y.(P(X,Y) ∧ Q(X) ∧ ¬R(Y))

Skolem:

∀Y.(P(c,Y) ∧ Q(c) ∧ ¬R(Y))

Causal:
{{P(c,Y)},{Q(c)},{¬R(Y)}}
```

### V:
```prolog
∀X.(P(X) ∧ ∃Y.(Q(Y) ∨ ∀Z.∃W.(P(Z) ∧ ¬Q(W))))

Skolem:
∀X.(P(X) ∧ ((Q(f(X)) v ∀Z.∃W.(P(Z) ∧ ¬Q(W))))) =

∀X.∀Z.P(X) ∧ (Q(f(X)) v (P(Z) ∧ ¬Q(g(X,Z))))   =

∀X.∀Z.P(X) ∧ ((Q(f(X)) v P(Z)) ∧ (Q(f(X)) v ¬Q(g(X,Z)))) 


Causal:
{{P(X)}, {Q(f(X)),P(Z)},{Q(f(X)),¬Q(g(X,Z))}}
```