## Absurdo clásico: (¬τ ⇒ ⊥) ⇒ τ
```
________Ax   _____Ax
Γ ⊢ ¬τ ⇒ ⊥   Γ ⊢ ¬τ
___________________⇒e
       Γ ⊢ ⊥
___________________PBC
    ¬τ ⇒ ⊥ ⊢ τ
___________________⇒i
   ⊢ (¬τ ⇒ ⊥) ⇒ τ

Γ = ¬τ ⇒ ⊥, ¬τ
```
## Ley de Peirce: ((τ ⇒ ρ) ⇒ τ ) ⇒ τ
```

                                                         _________Ax   _________Ax
                                                         Γ'', τ ⊢ τ    Γ'', τ ⊢ ¬τ
                                                         ____________________¬e
                                                         Γ'', τ ⊢ ⊥
                                                         _________⊥e
                                                         Γ'', τ ⊢ ρ
                                                         ___________⇒i   ____________Ax
                                                         Γ'' ⊢ (τ ⇒ ρ)   Γ'' ⊢ ¬(τ ⇒ ρ)
                         ______________Ax  ________Ax    _____________________________¬e
                         Γ' ⊢ (τ ⇒ ρ) ⇒ τ  Γ' ⊢ τ ⇒ ρ              Γ'' ⊢ ⊥
____________________LEM  _______________⇒e                     ______________PBC
Γ ⊢ (τ ⇒ ρ) v ¬(τ ⇒ ρ)   Γ, (τ ⇒ ρ) ⊢ τ                        Γ, ¬(τ ⇒ ρ) ⊢ τ
_______________________________________________________________________________ve
                                Γ ⊢ τ
                 ________________________________⇒i
                       ⊢ ((τ ⇒ ρ) ⇒ τ ) ⇒ τ

Γ = (τ ⇒ ρ) ⇒ τ
Γ' = (τ ⇒ ρ) ⇒ τ, (τ ⇒ ρ)
Γ'' = (τ ⇒ ρ) ⇒ τ, ¬(τ ⇒ ρ), ¬τ
```
## Tercero excluido: τ ∨ ¬τ

```
___________MORGAN I                            ___________MORGAN I
⊢ ¬(τ ∨ ¬τ) ⇒ ¬τ ∧ τ                           ⊢ ¬(τ ∨ ¬τ) ⇒ ¬τ ∧ τ
______________________WK      ____________Ax   ____________________WK  ____________Ax
Γ ⊢ ¬(τ ∨ ¬τ) ⇒ ¬τ ∧ τ        Γ ⊢ ¬(τ ∨ ¬τ)    Γ ⊢ ¬(τ ∨ ¬τ) ⇒ ¬τ ∧ τ  Γ ⊢ ¬(τ ∨ ¬τ)
___________________________________________⇒e  ________⇒e
               Γ ⊢ ¬τ ∧ τ                      Γ ⊢ ¬τ ∧ τ
__________________________∧e1                  ______ ∧e2
            Γ ⊢ τ                              Γ ⊢ ¬τ
___________________________________________________¬e
                    Γ ⊢ ⊥
________________________________PBC
                  ⊢ τ ∨ ¬τ

Γ = ¬(τ ∨ ¬τ)
```

## Consecuencia milagrosa: (¬τ ⇒ τ ) ⇒ τ
```


________Ax   _____Ax
Γ ⊢ ¬τ ⇒ τ   Γ ⊢ ¬τ
___________________⇒e      _____Ax
       Γ ⊢ τ               Γ ⊢ ¬τ
_________________________________¬e
         ¬τ ⇒ τ, ¬τ ⊢ ⊥
____________________________PBC
          ¬τ ⇒ τ ⊢ τ
_______________________⇒i
      ⊢ (¬τ ⇒ τ ) ⇒ τ

Γ = ¬τ ⇒ τ, ¬τ
```
## Contraposición clásica: (¬ρ ⇒ ¬τ ) ⇒ (τ ⇒ ρ)

```         

            _____________Ax  ________Ax
            Γ,¬ρ ⊢ ¬ρ ⇒ ¬τ   Γ,¬ρ ⊢ ¬ρ
______Ax    ___________________________⇒e
Γ,¬ρ ⊢ τ            Γ,¬ρ ⊢ ¬τ
______________________________¬e
           Γ,¬ρ ⊢ ⊥
____________________PBC
      Γ ⊢ ρ
______________⇒i
¬ρ ⇒ ¬τ ⊢ τ ⇒ ρ
______________________⇒i
 ⊢ (¬ρ ⇒ ¬τ ) ⇒ (τ ⇒ ρ)

Γ = ¬ρ ⇒ ¬τ, τ

```

## Análisis de casos: (τ ⇒ ρ) ⇒ (¬τ ⇒ ρ) ⇒ ρ


