## 1.1
$(\neg P \vee Q) \equiv \neg True \vee True \equiv True$ 

## 1.2
$(P \vee (S \land T) \vee Q) \equiv (True \vee (False \land False) \vee True) \equiv True$

## 1.3
$\neg (Q \vee S) \equiv \neg (True \vee False) \equiv \neg True \equiv False$

## 1.4
$$(\neg P \vee S) \Leftrightarrow (\neg P \land \neg S) \equiv$$
$$(\neg True \vee False) \Leftrightarrow (\neg True \land \neg False) \equiv$$
$$False \Leftrightarrow False \equiv$$
$$True$$

## 1.5
$$((P \vee S) \land (T \land Q)) \equiv$$
$$((True \vee False) \land (False \land True)) \equiv$$ 
$$(True \land False) \equiv$$ 
$$False$$

## 1.6

