## I: λz . if z then zero else succ(zero)
```
Paso 1: Esta rectificado.
Paso 2:  Γ = ∅, M = λz:X1. if z then zero else succ(zero)
Paso 3:
I(∅| λz:X1. if z then zero else succ(zero)) = (X1 -> Nat| {X1 =? Bool})
    I(z:X1 | if z then zero else succ(zero)) = (Nat | {X1 =? Bool, Nat =? Nat})
        I(z:X1 | z)         = (X1 | ∅)
        I(z:X1 | zero)      = (Nat | ∅)
        I(z:X1 | suc(zero)) = (Nat| Nat =? Nat)
            I(z:X1 | zero) = (Nat | ∅)
Paso 3: S = mgu({X1 =? Bool}) 
        S = {X1:= Bool}   

S(Γ) ⊢ S(M) : S(τ) = ∅ ⊢ λz:Bool. if z then zero else succ(zero) : Bool -> Nat
```