## a) Reglas de tipado:
```

Γ ⊢ M : σ  Γ ⊢ N : τ            Γ ⊢ M : σ × τ         Γ ⊢ M : σ × τ
___________________ t-par       _____________t-pi1    ______________t-pi2
Γ ⊢ 〈M, N〉 : σ × τ              Γ ⊢ π1(M) : σ         Γ ⊢ π2(M) : τ

```
### I: Constructor de pares: σ → τ → (σ × τ)
```

__________________Ax  _________________Ax
Γ, x:σ, y:τ ⊢ x : σ   Γ, x:σ, y:τ ⊢ y : τ
_________________________________________t-par
    Γ, x:σ, y:τ ⊢ 〈x, y〉 : σ × τ
____________________________________t-abs
 Γ, x:σ ⊢ λy:τ. 〈x, y〉 : τ → (σ × τ)
_____________________________________t-abs
Γ ⊢ λx:σ.λy:τ. 〈x, y〉 : σ → τ → (σ × τ)
```
### II: (σ × τ ) → σ y (σ × τ ) → τ
```
_______________________Ax
Γ , x : σ × τ ⊢ x : σ × τ
__________________________t-pi1
Γ ,x : σ × τ ⊢  π1(x) : σ
_________________________________t-abs
Γ ⊢ λx: σ × τ. π1(x) : (σ × τ ) → σ


_______________________Ax
Γ , x : σ × τ ⊢ x : σ × τ
__________________________t-pi1
Γ ,x : σ × τ ⊢  π2(x) : τ
_________________________________t-abs
Γ ⊢ λx: σ × τ. π2(x) : (σ × τ ) → τ
```
### Conmutatividad: (σ × τ ) → (τ × σ)
```
_____________________Ax         _____________________Ax
Γ ,x :σ × τ ⊢ x : σ × τ         Γ ,x :σ × τ ⊢ x : σ × τ 
________________________t-pi2   __________________t-pi1
Γ ,x :σ × τ ⊢ π2(x): τ          Γ ,x :σ × τ ⊢ π1(x): σ
________________________________________________t-par
Γ ,x :σ × τ ⊢  〈π2(x), π1(x)〉 : τ × σ
_____________________________________________t-abs
Γ ⊢ λx:σ × τ. 〈π2(x), π1(x)〉 : (σ × τ ) → τ × σ

```

## Asociatividad: ((σ × τ ) × ρ) → (σ × (τ × ρ))
```    
                        ____________________Ax
                        Γ' ⊢ x : (σ × τ) × ρ
___________________Ax   ____________________t-π1   __________________Ax
Γ' ⊢ x : (σ × τ) × ρ    Γ' ⊢ π1(x) : σ × τ         Γ' ⊢ x : (σ × τ) × ρ 
_______________t-π1     _______________t-π1        ____________t-π2
Γ' ⊢ π1(x): σ × τ       Γ' ⊢ π2(π1(x)) :τ          Γ' ⊢ π2(x) : ρ
_______________t-π1     __________________________________________t-par
Γ' ⊢ π1(π1(x)) : σ            Γ' ⊢ 〈π2(π1(x)), π2(x)〉: τ × ρ
___________________________________________________________________t-par
        Γ' ⊢ 〈π1(π1(x)), 〈π2(π1(x)), π2(x)〉〉: σ × (τ × ρ)
_____________________________________________________________________________t-abs
Γ ⊢ λx:(σ × τ) × ρ. 〈π1(π1(x)), 〈π2(π1(x)), π2(x)〉〉 : (σ × τ ) × ρ → σ × (τ × ρ)

Γ' = Γ U {x: (σ × τ) × ρ}

```
