## Reglas de tipado.
τ ::= . . . | [τ]
M, N, O ::= . . . | [ ]τ | M :: N | case M of {[ ] ; N | h :: t ; O} 
                  | foldr M base ; N ; rec(h, r) ; O
```haskell
__________t-vacia
Γ ⊢ [ ]τ: [τ]


Γ ⊢ M: τ  Γ ⊢ N: [τ]
___________________t-lista
  Γ ⊢ M :: N: [τ]


Γ ⊢ M: [τ]  Γ ⊢ N: ρ  Γ, h: τ, t: [τ] ⊢ O: ρ
____________________________________________t-case
Γ ⊢ case M of {[ ] ; N | h :: t ; O} : ρ


Γ ⊢ M: [τ]  Γ ⊢ N: ρ  Γ, h: τ, r: ρ ⊢ O: ρ
__________________________________________t-fold
Γ ⊢ foldr M base ; N ; rec(h, r) ; O: ρ
```

### Demostrar: 
```haskell
            ________ax   __________ax
            Γ ⊢ x: Bool  Γ ⊢ y:[Bool]
_________ax ______________t-lista       __________ax  ____________ax  __________________ax
Γ ⊢ x: Bool Γ ⊢ x :: y: [Bool]          Γ' ⊢ h: Bool  Γ' ⊢ r: [Bool]  Γ' ⊢ [ ]Bool: [Bool]
___________________t-lista ___________ax  _____________________________________________t-if
Γ ⊢ x :: x :: y: [Bool]    Γ ⊢ y: [Bool]  Γ, h: Bool, r: [Bool] ⊢ if h then r else [ ]Bool: [Bool]
_____________________________________________________________________________________t-fold
Γ = x : Bool, y : [Bool] ⊢ foldr x :: x :: y base ; y; rec(h, r) ; if h then r else [ ]Bool : [Bool]

```
### Lo valore:
V ::== ... | [ ]τ | V :: V

## Reglas de reducción:
M, N, O ::= . . . | [ ]τ | M :: N | case M of {[ ] ; N | h :: t ; O} 
                  | foldr M base ; N ; rec(h, r) ; O

```haskell

    M --> M'
__________________e-lista1
M :: N --> M' :: N

    N --> N'
_________________e-lista2
V :: N --> V :: N'
                              M --> M'
___________________________________________________________________e-case1
case M of {[ ] ; N | h :: t ; O} --> case M' of {[ ] ; N | h :: t ; O}

________________________________________e-case2
case [ ]τ of {[ ] ; N | h :: t ; O} --> N
________________________________________________________e-case3
case V1 :: V2 {[ ] ; N | h :: t ; O} --> O{h:= V1}{t:= V2}

                             M --> M'
________________________________________________________________e-fold1
foldr M base ; N ; rec(h, r) ; O --> foldr M' base ; N ; rec(h, r) ; O

                                        e-fold2
foldr [ ]τ base ; N ; rec(h, r) ; O --> N
                                                          e-fold3
foldr V1 :: V2 base ; N ; rec(h, r) ; O --> O{h:= V1}{r:= V2}
```