## A: σ → τ → σ

```haskell

_________________t-var
x: σ, y: τ ⊢ x: σ
________________________t-abs
x: σ ⊢ λy: τ. x: τ → σ
_______________________________t-abs
⊢ (λx :σ. (λy: τ. x)): σ → τ → σ 
```
## B: (σ → τ → ρ) → (σ → τ) → σ → ρ
```haskell
_____________t-var ______t-var   ________t-var  ______t-var
Γ ⊢ f: σ → τ → ρ   Γ ⊢ x: σ      Γ ⊢ g:σ → τ    Γ ⊢ x: τ
______________t-app              __________t-app
Γ ⊢ f x: τ → ρ                   Γ ⊢ g x: τ
_____________________________________________t-app
Γ = f: σ → τ → ρ, g : σ → τ, x : σ ⊢ f x (g x): ρ
_________________________________________t-abs
f: σ → τ → ρ, g : σ → τ ⊢ λx : σ. f x (g x): σ → ρ
____________________________________________________________t-abs
f: σ → τ → ρ ⊢ λg : σ → τ. λx : σ. f x (g x): (σ → τ) → σ → ρ
______________________________________________________________________________t-abs
⊢ λf : σ → τ → ρ. λg : σ → τ. λx : σ. f x (g x): (σ → τ → ρ) → (σ → τ) → σ → ρ

```
## C: (σ → τ → ρ) → τ → σ → ρ
```haskell



```