## ∀ p::(a,b) . intercambiar (intercambiar p) = p
```haskell
{I} : intercambiar (x,y) = (y,x)

-- Por lema de generacion de pares:
-- ∃x::a. ∃y::b. p = (x,y).

-- Qvq:
intercambiar (intercambiar (x,y)) = (x,y) 
intercambiar (y,x) = (x,y) ≡ por {I}
(x,y) = (x,y) ≡ por {I}   

```
## ∀ p::(a,(b,c)) . asociarD (asociarI p) = p
```haskell

{AD} : asociarD ((x,y),z) = (x,(y,z))
{AI} : asociarI (x,(y,z)) = ((x,y),z)

-- Por lema de generacion de pares:
-- ∃x::a. ∃y::b. ∃z::c. p = (x,(y,z)).

-- Qvq: 
asociarD (asociarI (x,(y,z))) = (x,(y,z)) 
asociarD ((x,y),z) = (x,(y,z)) ≡ por {AI}
(x,(y,z)) = (x,(y,z)) ≡ por {AD}  
```
## ∀ p::Either a b . espejar (espejar p) = p
```haskell
{EL} : espejar (Left x) = Right x
{ER} : espejar (Right x) = Left x

-- Por lema de generacion de suma:
-- o bien ∃x :: a. p = Left x
-- o bien ∃y :: b. p = Right y

-- Caso p = Left x
espejar (espejar (Left x)) = Left x
espejar (Right x) = Left x ≡ por {EL}
Left x = Left x ≡ por {ER}

-- Caso p = Right y
espejar (espejar (Right y)) = Right y
espejar (Left y) = Right y ≡ por {ER}
Right y = Right y ≡ por {EL}
```

## ∀ f::a->b->c . ∀ x::a . ∀ y::b . flip (flip f) x y = f x y
```haskell
{F} : flip f x y = f y x

flip (flip f) x y = f x y 
(flip f) y x = f x y ≡ por {F}
f x y = f x y ≡ por {F}
```
## ∀ f::a->b->c . ∀ x::a . ∀ y::b . curry (uncurry f) x y = f x y
```haskell
{C} curry f x y = f (x,y)
{U} uncurry f (x,y) = f x y

curry (uncurry f) x y = f x y 
uncurry f (x,y) = f x y ≡ por {C}
f x y = f x y ≡ por {U}
```
