## ∀ x::AB a . altura x ≤ cantNodos x
```haskell
-- Definiciones:

data AB a = Nil | Bin (AB a) a (AB a)
-- foldAB :: (b -> a -> b -> b) -> b -> AB a -> b
{F0} foldAB f z Nil = z
{F1} foldAB f z (Bin izq dato der) = f (foldAB f z izq) dato (foldAB f z der)

-- altura :: AB a -> Int
{A} altura x = foldAB (\izq r der -> 1 + max izq der) 0 x

-- cantNodos :: AB a -> Int 
{C} cantNodos x = foldAB (\izq r der -> 1 + izq + der) 0 x

-- Usando induccion estructural en x quiero ver que valen:

1) Caso Base. P(Nil)
2) Caso Inductivo. ∀ i, d :: AB a. ((P(i) && P(d)) => P(Bin i r d))

Con P(x) ≡ ∀ x::AB a . altura x ≤ cantNodos x

-- Caso Base. P(Nil)
altura Nil ≤ cantNodos Nil
foldAB (\izq r der -> 1 + max izq der) 0 Nil ≤ cantNodos Nil ≡ por {A}
0 ≤ cantNodos Nil ≡ por {F0}
0 ≤ foldAB (\izq r der -> 1 + izq + der) 0 Nil ≡ por {C}
0 ≤ 0 ≡ por {F0}

-- Caso Inductivo. ((P(i) && P(d)) => P(Bin i r d))

-- Sea
P(i) ≡ ∀ i::AB a. altura i ≤ cantNodos i
P(d) ≡ ∀ d::AB a. altura d ≤ cantNodos d

-- Qvq P(Bin i d)
altura (Bin i r d) ≤ cantNodos (Bin i r d)
foldAB (\izq _ der -> 1 + max izq der) 0 (Bin i r d) ≤ cantNodos (Bin i r d)       ≡ por {A}
{- LLamo f = (\izq _ der -> 1 + max izq der) -}
f (foldAB f 0 i) r (foldAB f 0 d) ≤ cantNodos (Bin i r d)                          ≡ por {F1}
f (altura i) r (altura d) ≤ cantNodos (Bin i r d)                                  ≡ por {A}
1 + max (altura i) (altura d) ≤ cantNodos (Bin i r d)                              ≡ por {β}
1 + max (altura i) (altura d) ≤ foldAB (\izq r der -> 1 + izq + der) 0 (Bin i r d) ≡ por {C}
{- LLamo g = (\izq r der -> 1 + izq + der) -}
1 + max (altura i) (altura d) ≤ g (foldAB g 0 i) r (foldAB g 0 d)                  ≡ por {F1}
1 + max (altura i) (altura d) ≤ g (cantNodos i) r (cantNodos d)                    ≡ por {C}
1 + max (altura i) (altura d) ≤ 1 + (cantNodos i) + (cantNodos d)                  ≡ por {β}
max (altura i) (altura d) ≤ (cantNodos i) + (cantNodos d)                         ≡ por {Int}
{- 
   Por {HI} altura x ≤ cantNodos x 
   Asumiendo que ∀ x::AB a. altura x >= 0 y cantNodos x >= 0.
   Por Int altura i ≤ cantNodos i + cantNodos d
   Idem con altura d ≤ cantNodos i + cantNodos d
   Por lo tanto max (altura i) (altura d) ≤ cantNodos i + cantNodos d
-}
```