## Ejercicio 3:
Sea σ = ∃X.P(Y, Z) ∧ ∀Y.¬Q(Y, X) ∨ P(Y, Z)
```
I: fv(σ) = {Y,Z,X}
II:
σ{X:= W} = ∃X.P(Y, Z) ∧ ∀Y.¬Q(Y, W) ∨ P(Y, Z)
σ{Y:= W} = ∃X.P(W, Z) ∧ ∀Y.¬Q(Y, X) ∨ P(W, Z)
σ{Y:= f(X)} = ∃X.P(Y, f(X)) ∧ ∀Y.¬Q(Y, X) ∨ P(f(X), Z)
              Aca f(X), X queda ligada cuando era libre, renombramos
              ∃W.P(Y, f(X)) ∧ ∀Y.¬Q(f(X), X) ∨ P(f(X), Z)
{Z:= g(Y, Z)} = ∃X.P(Y, g(Y, Z)) ∧ ∀Y.¬Q(Y, X) ∨ P(Y, g(Y, Z))
```
## Ejercicio 4:
Dada σ = ¬∀X.(∃Y.P(X, Y, Z)) ∧ ∀Z.P(X, Y, Z)
```
I: fv(σ) = {Z, X, Y}
   ¬fv(σ) = {X, Y, Z}

II: Sea t = g(f(g(Y, Y)), Y).
σ{X := t} = ¬∀X.(∃Y.P(X, Y, Z)) ∧ ∀Z.P(t, Y, Z)
σ{Y := t} = ¬∀X.(∃Y.P(X, Y, Z)) ∧ ∀Z.P(X, t, Z)
σ{Z := t} = ¬∀X.(∃Y.P(X, Y, t)) ∧ ∀Z.P(X, Y, Z)
            Aca ∃Y captura variables de t, renombramos.
            ¬∀X.(∃W.P(X, W, t)) ∧ ∀Z.P(X, Y, Z)

III: Sea t = g(f(g(Y, Y)), Y)
σ{X := t, Y := t, Z := t} = ¬∀T.(∃W.P(T, W, t)) ∧ ∀Z.P(t, t, Z)

IV: Sea t = g(f(g(Y, Y)), Y)
σ({X := t} ◦ {Y := t} ◦ {Z := t}) = 
((σ{Z:=t}){Y:=t}){X:=t} = (¬∀X.(∃W.P(X, W, t)) ∧ ∀Z.P(X, Y, Z){Y:=t}){X:=t} =
                           ¬∀X.(∃W.P(X, W, t)) ∧ ∀Z.P(X, t, Z){X:=t} = 
                           ¬∀X.(∃W.P(X, W, t)) ∧ ∀Z.P(t, t, Z)
```