```
==> )
_______________________________ax
∀X.∀Y.P (X, Y) |- ∀X.∀Y.P (X, Y)
____________________________∀e
∀X.∀Y.P (X, Y) |- ∀Y.P (X, Y)
_________________________∀e
∀X.∀Y.P (X, Y) |- P (X, Y)
____________________________∀i
∀X.∀Y.P (X, Y) |- ∀X.P (X, Y)
__________________________________∀i
∀X.∀Y.P (X, Y) |- ∀Y.∀X.P (X, Y)
__________________________________->i
∀X.∀Y.P (X, Y ) => ∀Y.∀X.P (X, Y ).

<== )
_______________________________ax
∀Y.∀X.P (X, Y) |- ∀Y.∀X.P (X, Y)
____________________________∀e
∀Y.∀X.P (X, Y) |- ∀X.P (X, Y)
_________________________∀e
∀Y.∀X.P (X, Y) |- P (X, Y)
____________________________∀i
∀Y.∀X.P (X, Y) |- ∀Y.P (X, Y)
__________________________________∀i
∀Y.∀X.P (X, Y) |- ∀X.∀Y.P (X, Y)
_______________________________->i
∀Y.∀X.P (X, Y) => ∀X.∀Y.P (X, Y)


                       ____________________________ax 
                       R, ∀Y.P(X, Y) |- ∀Y.P (X, Y) 
                       _______________________∀E
                       R, ∀Y.P(X, Y) |- P(X,Y) 
_________________ax    ___________________________∃i
R |- ∃X.∀Y.P(X, Y)    R, ∀Y.P(X, Y) |- ∃X.P(X, Y)
___________________∃e
R |- ∃X.P(X, Y)
_________________________________∀i
R = {∃X.∀Y.P(X, Y)} |- ∀Y.∃X.P(X, Y )
_________________________________->i
∃X.∀Y.P(X, Y) => ∀Y.∃X.P(X, Y ).
```