```haskell

Γ ⊢ Δt   Γ ⊢ Δ¬t                       Γ, Δ¬t ⊢ t
________________Δe                     ___________Δi
     Γ ⊢ t                               Γ ⊢ Δt

⊢ t => Δt            
 
          ___________ax
          Γ, Δ¬¬t ⊢ ¬t
____ax    _________Δi
Γ ⊢ Δt    Γ ⊢ Δ¬t
___________________Δe     _____ax
      Γ ⊢ t               Γ ⊢ ¬t
_________________________________¬e
               Γ ⊢ ⊥          
_____________________¬i
Δt, Δ¬¬¬t ⊢ ¬¬t
________________Δi
Δt ⊢ Δ¬¬t

Γ = Δt, Δ¬¬¬t, ¬t   

                                         ________ax anterior 
                                         Δt ⊢ Δ¬¬t 
_____ax   _____ax            ______ax    _______weak
Γ ⊢ Δt    Γ ⊢ Δ¬t            Γ ⊢ Δ¬t     Γ ⊢ Δ¬¬t
__________________Δe         _____Δe
    Γ ⊢ t                    Γ ⊢ ¬t
____________________________________¬e
               Γ ⊢ ⊥
______________________⊥e
Δt, Δ¬t ⊢ q

Γ = Δt, Δ¬t
```